Added scanner and a Main routine. Programs Example0.source (which is intentially empty) and Example1.source successfully parse.

SourceParser.dfy
@@ -1,9 +1,5 @@
 include "SourceSyntax.dfy"
 
-extern "SourceScanner.Read"
-method SourceScannerRead() returns (stringTokens: array<string>)
-  ensures stringTokens != null
-
 function method IdToString(id: Id): string
 {
   if id <= 0 then "0" else
@@ -61,11 +57,12 @@ class Parser {
     stringTokens != null &&
     p <= stringTokens.Length
   }
-  constructor ()
+  constructor (tokens: array<string>)
+    requires tokens != null
     modifies this
     ensures Valid()
   {
-    stringTokens := SourceScannerRead();
+    stringTokens := tokens;
     p := 0;
   }
   function method Next(): string
