Main.dfy
@@ -1,0 +1,22 @@
+include "SourceScanner.dfy"
+include "SourceParser.dfy"
+
+extern "InputRead"
+method InputRead() returns (input: array<char>)
+  ensures input != null
+  decreases *
+
+method Main()
+  decreases *
+{
+  var chars := InputRead();
+  var stringTokens := SourceScannerRead(chars);
+  var parser := new Parser(stringTokens);
+  var success, prog := parser.Parse();
+  if success {
+    print "Parse succeeded!\n";
+    print prog, "\n";  // this may not be pretty
+  } else {
+    print "Parse failed :(\n";
+  }
+}
